reconstruct symbol table generation

assembler/Symbtablegen.v
@@ -1,10 +1,3 @@
-(* *******************  *)
-(* Author: Yuting Wang  *)
-(*         Jinhua Wu    *)
-(* Date:   Sep 13, 2019 *)
-(* Last updated: Feb 24, 2022 by Jinhua Wu *)
-(* *******************  *)
-
 Require Import Coqlib Integers AST Maps.
 Require Import Asm.
 Require Import Errors.
@@ -12,6 +5,7 @@ Require Import Memtype.
 Require Import RelocProg RelocProgram.
 Require Import CheckDef.
 Require Import LocalLib.
+Require Import SymbtablegenArchi.
 Require Globalenvs.
 Import ListNotations.
 
@@ -147,124 +141,7 @@ Definition gen_symb_table defs :=
   rstbl.
 
 
-(* End WITH_PROG_SECS. *)
-
-
-(** Check if the source program is well-formed **)
-
-(* Definition def_size (def: AST.globdef Asm.fundef unit) : Z := *)
-(*   match def with *)
-(*   | AST.Gfun (External e) => 1 *)
-(*   | AST.Gfun (Internal f) => Asm.code_size (Asm.fn_code f) *)
-(*   | AST.Gvar v => AST.init_data_list_size (AST.gvar_init v) *)
-(*   end. *)
-
-(* Definition odef_size (def: option (AST.globdef Asm.fundef unit)) : Z := *)
-(*   match def with *)
-(*   | Some def => def_size def *)
-(*   | _ => 0 *)
-(*   end. *)
-
-(* Lemma def_size_pos: *)
-(*   forall d, *)
-(*     0 <= def_size d. *)
-(* Proof. *)
-(*   unfold def_size. intros. *)
-(*   destr. *)
-(*   destr. generalize (code_size_non_neg (Asm.fn_code f0)); lia. *)
-(*   lia. *)
-(*   generalize (AST.init_data_list_size_pos (AST.gvar_init v)); lia. *)
-(* Qed. *)
-
-(* Lemma odef_size_pos: *)
-(*   forall d, *)
-(*     0 <= odef_size d. *)
-(* Proof. *)
-(*   unfold odef_size. intros. *)
-(*   destr. apply def_size_pos. lia. *)
-(* Qed. *)
-
-(* Definition def_not_empty def : Prop := *)
-(*   match def with *)
-(*   | None => True *)
-(*   | Some def' => 0 < def_size def' *)
-(*   end. *)
-
-
-(* Definition defs_not_empty defs := *)
-(*   Forall def_not_empty defs. *)
-
-(* Definition defs_not_empty_dec defs : { defs_not_empty defs } + { ~ defs_not_empty defs }. *)
-(* Proof. *)
-(*   apply Forall_dec. intros. destruct x.  *)
-(*   - simpl. apply zlt. *)
-(*   - simpl. left. auto. *)
-(* Defined. *)
-
-Definition main_exists main (defs: list (ident * (AST.globdef Asm.fundef unit))) :=
-  Exists (fun '(id, def) => 
-            main = id ) defs.
-
-Definition main_exists_dec main defs : {main_exists main defs } + {~ main_exists main defs}.
-Proof.
-  apply Exists_dec. intros. destruct x.
-  generalize (ident_eq main i). intros.
-  inv H.
-  - left. auto.
-  - right. inversion 1. auto.
-Qed.
-
-Local Open Scope Z_scope.
-
-Definition def_aligned (def: (globdef fundef unit)) :=
-  match def with
-  | (Gvar v) =>
-    match gvar_init v with
-    | nil
-    | [Init_space _] => True
-    | _ => (AST.init_data_list_size (gvar_init v)) mod alignw = 0
-    end
-  | (Gfun f) =>
-    match f with
-    | External _ => True
-    | Internal f => (code_size instr_size (fn_code f)) mod alignw = 0
-    end
-  end.
-
-Lemma def_aligned_dec: forall def, {def_aligned def} + {~def_aligned def}.
-Proof.
-  destruct def. 
-  - destruct f. 
-    + simpl. decide equality; decide equality.
-    + simpl. auto.
-  - simpl. destruct (gvar_init v); simpl. auto.
-    destruct i; try (decide equality; decide equality).
-    destruct l; auto.
-    decide equality; decide equality.
-Qed.
-    
-Definition instr_invalid (i: instruction) := 
-  match i with
-  | Pjmp_l _ 
-  | Pjcc _ _ 
-  | Pjcc2 _ _ _ 
-  (*Remove this instr after symbol table gen*)
-  | Pjmptbl _ _
-  | Pjmptbl_rel _ _
-  | Pallocframe _ _ _
-  | Pfreeframe _ _ _ => True
-  (* | Pload_parent_pointer _ _ _ => True *)
-  | _ => False
-  end.
-
-
 (** Create the code section *)
-Definition get_def_instrs (def: (globdef fundef unit)) : code :=
-  match def with
-  | (Gfun (Internal f)) => fn_code f
-  | _ => []
-  end.
-
 Definition acc_gen_section (acc: sectable) (iddef: ident * (globdef fundef unit)) : sectable :=
   let (id, def) := iddef in
   match def with
@@ -285,50 +162,6 @@ Definition acc_gen_section (acc: sectable) (iddef: ident * (globdef fundef unit)
 Definition create_sec_table (defs : list (ident * (globdef fundef unit))) : sectable :=
   fold_left acc_gen_section defs (PTree.empty section).
 
-Definition instr_valid i := ~instr_invalid i.
-
-Lemma instr_invalid_dec: forall i, {instr_invalid i} + {~instr_invalid i}.
-Proof.
-  destruct i; cbn; auto.
-Qed.
-
-Lemma instr_valid_dec: forall i, {instr_valid i} + {~instr_valid i}.
-Proof.
-  unfold instr_valid.
-  destruct i; cbn; auto.
-Qed.
-
-Definition def_instrs_valid (def: (globdef fundef unit)) :=
-  match def with
-  | (Gvar v) => True
-  | (Gfun f) =>
-    match f with
-    | External _ => True
-    | Internal f =>  Forall instr_valid (fn_code f)
-    end
-  end.
-
-Lemma def_instrs_valid_dec: 
-  forall def, {def_instrs_valid def} + {~def_instrs_valid def}.
-Proof.
-  destruct def.
-  - destruct f. 
-    + simpl. apply Forall_dec. apply instr_valid_dec.
-    + simpl. auto.
-  - simpl. auto.
-Qed.
-
-Definition data_size_aligned (def: (globdef fundef unit)) :=
-  (alignw | init_data_list_size (get_def_init_data def)).
-
-Lemma data_size_aligned_dec: forall def,
-    {data_size_aligned def} + {~data_size_aligned def}.
-Proof.
-  intros.
-  unfold data_size_aligned.
-  apply Zdivide_dec.
-  (* unfold alignw. lia. *)
-Qed.
     
 Record wf_prog (p:Asm.program) : Prop :=
   {
@@ -360,7 +193,7 @@ Definition transf_program (p:Asm.program) : res program :=
   if check_wellformedness p then
     let symb_tbl := gen_symb_table (AST.prog_defs p) in
     let sec_tbl := create_sec_table (AST.prog_defs p) in
-    if zle (sections_size instr_size (map snd (PTree.elements sec_tbl))) Ptrofs.max_unsigned then
+    if zle (defs_size (map snd (AST.prog_defs p))) Ptrofs.max_unsigned then
       OK {| prog_defs := AST.prog_defs p;
             prog_public := AST.prog_public p;
             prog_main := AST.prog_main p;
@@ -370,7 +203,7 @@ Definition transf_program (p:Asm.program) : res program :=
             prog_senv := Globalenvs.Genv.to_senv (Globalenvs.Genv.globalenv p)
          |}
     else 
-      Error (msg "Size of sections too big")
+      Error (msg "Program too big")
   else
     Error (msg "Program not well-formed").
 
