assembler/MemoryAgree.v
@@ -1,0 +1,548 @@
+Require Import Coqlib Errors Maps.
+Require Import Integers Floats.
+Require Import Values Memory Events Globalenvs.
+Require Import LocalLib AsmInject Asm.
+Import ListNotations.
+
+
+(** *A new injection: remove the perm_inv from Memory.inject *)
+Record magree (f: meminj) (m1 m2: mem) : Prop :=
+  mk_magree {
+    ma_inj:
+      Mem.mem_inj f m1 m2;
+    ma_freeblocks:
+      forall b, ~(Mem.valid_block m1 b) -> f b = None;
+    ma_mappedblocks:
+      forall b b' delta, f b = Some(b', delta) -> Mem.valid_block m2 b';
+    ma_no_overlap:
+      Mem.meminj_no_overlap f m1;
+    ma_representable:
+      forall b b' delta ofs,
+      f b = Some(b', delta) ->
+      Mem.perm m1 b (Ptrofs.unsigned ofs) Max Nonempty \/ Mem.perm m1 b (Ptrofs.unsigned ofs - 1) Max Nonempty ->
+      delta >= 0 /\ 0 <= Ptrofs.unsigned ofs + delta <= Ptrofs.max_unsigned
+  }.
+
+(** Assumption about external calls.
+    These should be merged into common properties about external calls later. *)
+Axiom external_call_inject : forall ge j vargs1 vargs2 m1 m2 m1' vres1 t ef,
+    j = Mem.flat_inj (Mem.support m1) ->
+    Val.inject_list j vargs1 vargs2 ->
+    magree j m1 m2 ->
+    external_call ef ge vargs1 m1 t vres1 m1' ->
+    exists j' vres2 m2',
+      external_call ef ge vargs2 m2 t vres2 m2' /\
+      Val.inject j' vres1 vres2 /\ magree j' m1' m2' /\
+      inject_incr j j' /\
+      inject_separated j j' m1 m2 /\
+      j' = Mem.flat_inj (Mem.support m1').
+
+
+Axiom  external_call_valid_block: forall ef ge vargs m1 t vres m2 b,
+    external_call ef ge vargs m1 t vres m2 -> Mem.valid_block m1 b -> Mem.valid_block m2 b.
+
+(* copy from Memory *)
+
+(** The following lemmas establish the absence of machine integer overflow
+  during address computations. *)
+
+Lemma address_inject:
+  forall f m1 m2 b1 ofs1 b2 delta p,
+  magree f m1 m2 ->
+  Mem.perm m1 b1 (Ptrofs.unsigned ofs1) Cur p ->
+  f b1 = Some (b2, delta) ->
+  Ptrofs.unsigned (Ptrofs.add ofs1 (Ptrofs.repr delta)) = Ptrofs.unsigned ofs1 + delta.
+Proof.
+  intros.
+  assert (Mem.perm m1 b1 (Ptrofs.unsigned ofs1) Max Nonempty) by eauto with mem.
+  exploit ma_representable; eauto. intros [A B].
+  assert (0 <= delta <= Ptrofs.max_unsigned).
+    generalize (Ptrofs.unsigned_range ofs1). lia.
+  unfold Ptrofs.add. repeat rewrite Ptrofs.unsigned_repr; lia.
+Qed.
+
+Lemma address_inject':
+  forall f m1 m2 chunk b1 ofs1 b2 delta,
+  magree f m1 m2 ->
+  Mem.valid_access m1 chunk b1 (Ptrofs.unsigned ofs1) Nonempty ->
+  f b1 = Some (b2, delta) ->
+  Ptrofs.unsigned (Ptrofs.add ofs1 (Ptrofs.repr delta)) = Ptrofs.unsigned ofs1 + delta.
+Proof.
+  intros. destruct H0. eapply address_inject; eauto.
+  apply H0. generalize (size_chunk_pos chunk). lia.
+Qed.
+
+Theorem weak_valid_pointer_inject_no_overflow:
+  forall f m1 m2 b ofs b' delta,
+  magree f m1 m2 ->
+  Mem.weak_valid_pointer m1 b (Ptrofs.unsigned ofs) = true ->
+  f b = Some(b', delta) ->
+  0 <= Ptrofs.unsigned ofs + Ptrofs.unsigned (Ptrofs.repr delta) <= Ptrofs.max_unsigned.
+Proof.
+  intros. rewrite Mem.weak_valid_pointer_spec in H0.
+  rewrite ! Mem.valid_pointer_nonempty_perm in H0.
+  exploit ma_representable; eauto. destruct H0; eauto with mem.
+  intros [A B].
+  pose proof (Ptrofs.unsigned_range ofs).
+  rewrite Ptrofs.unsigned_repr; lia.
+Qed.
+
+Theorem valid_access_inject:
+  forall f m1 m2 chunk b1 ofs b2 delta p,
+  f b1 = Some(b2, delta) ->
+  magree f m1 m2 ->
+  Mem.valid_access m1 chunk b1 ofs p ->
+  Mem.valid_access m2 chunk b2 (ofs + delta) p.
+Proof.
+  intros. eapply Mem.valid_access_inj; eauto. apply ma_inj; auto.
+Qed.
+
+Theorem valid_pointer_inject:
+  forall f m1 m2 b1 ofs b2 delta,
+  f b1 = Some(b2, delta) ->
+  magree f m1 m2 ->
+  Mem.valid_pointer m1 b1 ofs = true ->
+  Mem.valid_pointer m2 b2 (ofs + delta) = true.
+Proof.
+  intros.
+  rewrite Mem.valid_pointer_valid_access in H1.
+  rewrite Mem.valid_pointer_valid_access.
+  eapply valid_access_inject; eauto.
+Qed.
+
+Theorem weak_valid_pointer_inject:
+  forall f m1 m2 b1 ofs b2 delta,
+  f b1 = Some(b2, delta) ->
+  magree f m1 m2 ->
+  Mem.weak_valid_pointer m1 b1 ofs = true ->
+  Mem.weak_valid_pointer m2 b2 (ofs + delta) = true.
+Proof.
+  intros until 2. unfold Mem.weak_valid_pointer. rewrite !orb_true_iff.
+  replace (ofs + delta - 1) with ((ofs - 1) + delta) by lia.
+  intros []; eauto using valid_pointer_inject.
+Qed.
+
+Theorem valid_pointer_inject_val:
+  forall f m1 m2 b ofs b' ofs',
+  magree f m1 m2 ->
+  Mem.valid_pointer m1 b (Ptrofs.unsigned ofs) = true ->
+  Val.inject f (Vptr b ofs) (Vptr b' ofs') ->
+  Mem.valid_pointer m2 b' (Ptrofs.unsigned ofs') = true.
+Proof.
+  intros. inv H1.
+  erewrite address_inject'; eauto.
+  eapply valid_pointer_inject; eauto.
+  rewrite Mem.valid_pointer_valid_access in H0. eauto.
+Qed.
+
+Theorem weak_valid_pointer_inject_val:
+  forall f m1 m2 b ofs b' ofs',
+  magree f m1 m2 ->
+  Mem.weak_valid_pointer m1 b (Ptrofs.unsigned ofs) = true ->
+  Val.inject f (Vptr b ofs) (Vptr b' ofs') ->
+  Mem.weak_valid_pointer m2 b' (Ptrofs.unsigned ofs') = true.
+Proof.
+  intros. inv H1.
+  exploit weak_valid_pointer_inject; eauto. intros W.
+  rewrite Mem.weak_valid_pointer_spec in H0.
+  rewrite ! Mem.valid_pointer_nonempty_perm in H0.
+  exploit ma_representable; eauto. destruct H0; eauto with mem.
+  intros [A B].
+  pose proof (Ptrofs.unsigned_range ofs).
+  unfold Ptrofs.add. repeat rewrite Ptrofs.unsigned_repr; auto; lia.
+Qed.
+
+(* copy from Asminject *)
+(** Injection for cmpu_bool and cmplu_bool *)
+Lemma valid_ptr_inj : forall j m m',
+    magree j m m' ->
+    forall b i b' delta,                                  
+      j b = Some (b', delta) ->
+      Mem.valid_pointer m b (Ptrofs.unsigned i) = true ->
+      Mem.valid_pointer m' b' (Ptrofs.unsigned (Ptrofs.add i (Ptrofs.repr delta))) = true.
+Proof.
+  intros. eapply valid_pointer_inject_val; eauto.
+Qed.
+
+
+Lemma weak_valid_ptr_inj: forall j m m',
+  magree j m m' ->
+  forall b1 ofs b2 delta,
+  j b1 = Some(b2, delta) ->
+  Mem.weak_valid_pointer m b1 (Ptrofs.unsigned ofs) = true ->
+  Mem.weak_valid_pointer m' b2 (Ptrofs.unsigned (Ptrofs.add ofs (Ptrofs.repr delta))) = true.
+Proof.
+  intros. eapply weak_valid_pointer_inject_val; eauto.
+Qed.
+
+Lemma weak_valid_ptr_no_overflow: forall j m m',
+  magree j m m' ->
+  forall b1 ofs b2 delta,
+  j b1 = Some(b2, delta) ->
+  Mem.weak_valid_pointer m b1 (Ptrofs.unsigned ofs) = true ->
+  0 <= Ptrofs.unsigned ofs + Ptrofs.unsigned (Ptrofs.repr delta) <= Ptrofs.max_unsigned.
+Proof.
+  intros. eapply weak_valid_pointer_inject_no_overflow; eauto.
+Qed.
+
+Theorem different_pointers_inject:
+  forall f m m' b1 ofs1 b2 ofs2 b1' delta1 b2' delta2,
+  magree f m m' ->
+  b1 <> b2 ->
+  Mem.valid_pointer m b1 (Ptrofs.unsigned ofs1) = true ->
+  Mem.valid_pointer m b2 (Ptrofs.unsigned ofs2) = true ->
+  f b1 = Some (b1', delta1) ->
+  f b2 = Some (b2', delta2) ->
+  b1' <> b2' \/
+  Ptrofs.unsigned (Ptrofs.add ofs1 (Ptrofs.repr delta1)) <>
+  Ptrofs.unsigned (Ptrofs.add ofs2 (Ptrofs.repr delta2)).
+Proof.
+  intros.
+  rewrite Mem.valid_pointer_valid_access in H1.
+  rewrite Mem.valid_pointer_valid_access in H2.
+  rewrite (address_inject' _ _ _ _ _ _ _ _ H H1 H3).
+  rewrite (address_inject' _ _ _ _ _ _ _ _ H H2 H4).
+  inv H1. simpl in H5. inv H2. simpl in H1.
+  eapply ma_no_overlap; eauto.
+  apply Mem.perm_cur_max. apply (H5 (Ptrofs.unsigned ofs1)). lia.
+  apply Mem.perm_cur_max. apply (H1 (Ptrofs.unsigned ofs2)). lia.
+Qed.
+
+Lemma valid_different_ptrs_inj: forall j m m',
+  magree j m m' ->
+  forall b1 ofs1 b2 ofs2 b1' delta1 b2' delta2,
+  b1 <> b2 ->
+  Mem.valid_pointer m b1 (Ptrofs.unsigned ofs1) = true ->
+  Mem.valid_pointer m b2 (Ptrofs.unsigned ofs2) = true ->
+  j b1 = Some (b1', delta1) ->
+  j b2 = Some (b2', delta2) ->
+  b1' <> b2' \/
+  Ptrofs.unsigned (Ptrofs.add ofs1 (Ptrofs.repr delta1)) <> Ptrofs.unsigned (Ptrofs.add ofs2 (Ptrofs.repr delta2)).
+Proof.
+  intros. eapply different_pointers_inject; eauto.
+Qed.
+
+Definition cmpu_bool_inject := fun j m m' (MINJ: magree j m m') =>
+                     Val.cmpu_bool_inject j (Mem.valid_pointer m) (Mem.valid_pointer m')
+                                          (valid_ptr_inj j m m' MINJ)
+                                          (weak_valid_ptr_inj j m m' MINJ)
+                                          (weak_valid_ptr_no_overflow j m m' MINJ)
+                                          (valid_different_ptrs_inj j m m' MINJ).
+
+Lemma cmpu_bool_lessdef : forall j v1 v2 v1' v2' m m' c,
+    Val.inject j v1 v1' -> Val.inject j v2 v2' ->
+    magree j m m' ->
+    Val.opt_lessdef (Val.cmpu_bool (Mem.valid_pointer m) c v1 v2)
+                (Val.cmpu_bool (Mem.valid_pointer m') c v1' v2').
+Proof.
+  intros. destruct (Val.cmpu_bool (Mem.valid_pointer m) c v1 v2) eqn:EQ.
+  - exploit (cmpu_bool_inject j m m' H1 c v1 v2); eauto.
+    intros. rewrite H2. constructor.
+  - constructor.
+Qed.
+
+Definition cmplu_bool_inject := fun j m m' (MINJ: magree j m m') =>
+                     Val.cmplu_bool_inject j (Mem.valid_pointer m) (Mem.valid_pointer m')
+                                           (valid_ptr_inj j m m' MINJ)
+                                           (weak_valid_ptr_inj j m m' MINJ)
+                                           (weak_valid_ptr_no_overflow j m m' MINJ)
+                                           (valid_different_ptrs_inj j m m' MINJ).
+
+
+Lemma cmplu_bool_lessdef : forall j v1 v2 v1' v2' m m' c,
+    Val.inject j v1 v1' -> Val.inject j v2 v2' ->
+    magree j m m' ->
+    Val.opt_lessdef (Val.cmplu_bool (Mem.valid_pointer m) c v1 v2)
+                (Val.cmplu_bool (Mem.valid_pointer m') c v1' v2').
+Proof.
+  intros. destruct (Val.cmplu_bool (Mem.valid_pointer m) c v1 v2) eqn:EQ.
+  - exploit (cmplu_bool_inject j m m' H1 c v1 v2); eauto.
+    intros. rewrite H2. constructor.
+  - constructor.
+Qed.
+
+Lemma cmpu_inject : forall j v1 v2 v1' v2' m m' c,
+    Val.inject j v1 v1' -> Val.inject j v2 v2' ->
+    magree j m m' ->
+    Val.inject j (Val.cmpu (Mem.valid_pointer m) c v1 v2)
+               (Val.cmpu (Mem.valid_pointer m') c v1' v2').
+Proof.
+  intros. unfold Val.cmpu.
+  exploit (cmpu_bool_lessdef j v1 v2); eauto. intros. 
+  exploit val_of_optbool_lessdef; eauto.
+Qed.
+
+
+Lemma cmplu_lessdef : forall j v1 v2 v1' v2' m m' c,
+    Val.inject j v1 v1' -> Val.inject j v2 v2' ->
+    magree j  m m' ->
+    Val.opt_val_inject j (Val.cmplu (Mem.valid_pointer m) c v1 v2)
+                     (Val.cmplu (Mem.valid_pointer m') c v1' v2').
+Proof.
+  intros. unfold Val.cmplu.
+  exploit (cmplu_bool_lessdef j v1 v2 v1' v2' m m' c); eauto. intros.
+  inversion H2; subst; simpl; constructor.
+  apply Val.vofbool_inject.
+Qed.
+(* end of copy *)
+
+Lemma compare_ints_inject: forall j v1 v2 v1' v2' rs rs' m m',
+    Val.inject j v1 v1' -> Val.inject j v2 v2' ->
+    magree j m m' ->
+    regset_inject j rs rs' -> 
+    regset_inject j (compare_ints v1 v2 rs m) (compare_ints v1' v2' rs' m').
+Proof.
+  intros. unfold compare_ints, Asm.compare_ints.
+  repeat apply regset_inject_expand; auto.
+  - apply cmpu_inject; auto.
+  - apply cmpu_inject; auto.
+  - apply val_negative_inject. apply Val.sub_inject; auto.
+  - apply sub_overflow_inject; auto.
+Qed.
+
+Lemma compare_longs_inject: forall j v1 v2 v1' v2' rs rs' m m',
+    Val.inject j v1 v1' -> Val.inject j v2 v2' ->
+    magree j m m' ->
+    regset_inject j rs rs' -> 
+    regset_inject j (compare_longs v1 v2 rs m) (compare_longs v1' v2' rs' m').
+Proof.
+  intros. unfold compare_longs, Asm.compare_longs.
+  repeat apply regset_inject_expand; auto.
+  - unfold Val.cmplu.
+    exploit (cmplu_bool_lessdef j v1 v2 v1' v2' m m' Ceq); eauto. intros.
+    inversion H3; subst.
+    + simpl. auto. 
+    + simpl. apply Val.vofbool_inject.
+  - unfold Val.cmplu.
+    exploit (cmplu_bool_lessdef j v1 v2 v1' v2' m m' Clt); eauto. intros.
+    inversion H3; subst.
+    + simpl. auto. 
+    + simpl. apply Val.vofbool_inject.
+  - apply val_negativel_inject. apply Val.subl_inject; auto.
+  - apply subl_overflow_inject; auto.
+Qed.
+
+
+(** Preservation of loads *)
+
+Theorem load_inject:
+  forall f m1 m2 chunk b1 ofs b2 delta v1,
+  magree f m1 m2 ->
+  Mem.load chunk m1 b1 ofs = Some v1 ->
+  f b1 = Some (b2, delta) ->
+  exists v2, Mem.load chunk m2 b2 (ofs + delta) = Some v2 /\ Val.inject f v1 v2.
+Proof.
+  intros. inv H. eapply Mem.load_inj; eauto.
+Qed.
+
+Theorem loadv_inject:
+  forall f m1 m2 chunk a1 a2 v1,
+  magree f m1 m2 ->
+  Mem.loadv chunk m1 a1 = Some v1 ->
+  Val.inject f a1 a2 ->
+  exists v2, Mem.loadv chunk m2 a2 = Some v2 /\ Val.inject f v1 v2.
+Proof.
+  intros. inv H1; simpl in H0; try discriminate.
+  exploit load_inject; eauto. intros [v2 [LOAD INJ]].
+  exists v2; split; auto. unfold Mem.loadv.
+  replace (Ptrofs.unsigned (Ptrofs.add ofs1 (Ptrofs.repr delta)))
+     with (Ptrofs.unsigned ofs1 + delta).
+  auto. symmetry. eapply address_inject'; eauto with mem.
+Qed.
+
+Theorem loadbytes_inject:
+  forall f m1 m2 b1 ofs len b2 delta bytes1,
+  magree f m1 m2 ->
+  Mem.loadbytes m1 b1 ofs len = Some bytes1 ->
+  f b1 = Some (b2, delta) ->
+  exists bytes2, Mem.loadbytes m2 b2 (ofs + delta) len = Some bytes2
+              /\ list_forall2 (memval_inject f) bytes1 bytes2.
+Proof.
+  intros. inv H. eapply Mem.loadbytes_inj; eauto.
+Qed.
+
+(** Preservation of stores *)
+
+Theorem store_mapped_inject:
+  forall f chunk m1 b1 ofs v1 n1 m2 b2 delta v2,
+  magree f m1 m2 ->
+  Mem.store chunk m1 b1 ofs v1 = Some n1 ->
+  f b1 = Some (b2, delta) ->
+  Val.inject f v1 v2 ->
+  exists n2,
+    Mem.store chunk m2 b2 (ofs + delta) v2 = Some n2
+    /\ magree f n1 n2.
+Proof.
+  intros. inversion H.
+  exploit Mem.store_mapped_inj; eauto. intros [n2 [STORE MI]].
+  exists n2; split. eauto. constructor.
+(* inj *)
+  auto.
+(* freeblocks *)
+  eauto with mem.
+(* mappedblocks *)
+  eauto with mem.
+(* no overlap *)
+  red; intros. eauto with mem.
+(* representable *)
+  intros. eapply ma_representable; try eassumption.
+  destruct H4; eauto with mem.
+Qed.
+
+
+Theorem storev_mapped_inject:
+  forall f chunk m1 a1 v1 n1 m2 a2 v2,
+  magree f m1 m2 ->
+  Mem.storev chunk m1 a1 v1 = Some n1 ->
+  Val.inject f a1 a2 ->
+  Val.inject f v1 v2 ->
+  exists n2,
+    Mem.storev chunk m2 a2 v2 = Some n2 /\ magree f n1 n2.
+Proof.
+  intros. inv H1; simpl in H0; try discriminate.
+  unfold Mem.storev.
+  replace (Ptrofs.unsigned (Ptrofs.add ofs1 (Ptrofs.repr delta)))
+    with (Ptrofs.unsigned ofs1 + delta).
+  eapply store_mapped_inject; eauto.
+  symmetry. eapply address_inject'; eauto with mem.
+Qed.
+
+
+(* Preservaiton of allocation *)
+Theorem alloc_left_mapped_inject:
+  forall f m1 m2 lo hi m1' b1 b2 delta,
+  magree f m1 m2 ->
+  Mem.alloc m1 lo hi = (m1', b1) ->
+  Mem.valid_block m2 b2 ->
+  0 <= delta <= Ptrofs.max_unsigned ->
+  (forall ofs k p, Mem.perm m2 b2 ofs k p -> delta = 0 \/ 0 <= ofs < Ptrofs.max_unsigned) ->
+  (forall ofs k p, lo <= ofs < hi -> Mem.perm m2 b2 (ofs + delta) k p) ->
+  Mem.inj_offset_aligned delta (hi-lo) ->
+  (forall b delta' ofs k p,
+   f b = Some (b2, delta') ->
+   Mem.perm m1 b ofs k p ->
+   lo + delta <= ofs + delta' < hi + delta -> False) ->
+  exists f',
+     magree f' m1' m2
+  /\ inject_incr f f'
+  /\ f' b1 = Some(b2, delta)
+  /\ (forall b, b <> b1 -> f' b = f b).
+Proof.
+  intros. inversion H.
+  set (f' := fun b => if eq_block b b1 then Some(b2, delta) else f b).
+  assert (inject_incr f f').
+    red; unfold f'; intros. destruct (eq_block b b1). subst b.
+    assert (f b1 = None). eauto with mem. congruence.
+    auto.
+  assert (Mem.mem_inj f' m1 m2).
+    inversion ma_inj0; constructor; eauto with mem.
+    unfold f'; intros. destruct (eq_block b0 b1).
+      inversion H8. subst b0 b3 delta0.
+      elim (Mem.fresh_block_alloc _ _ _ _ _ H0). eauto with mem.
+      eauto.
+    unfold f'; intros. destruct (eq_block b0 b1).
+      inversion H8. subst b0 b3 delta0.
+      elim (Mem.fresh_block_alloc _ _ _ _ _ H0).
+      eapply Mem.perm_valid_block with (ofs := ofs). apply H9. generalize (size_chunk_pos chunk); lia.
+      eauto.
+    unfold f'; intros. destruct (eq_block b0 b1).
+      inversion H8. subst b0 b3 delta0.
+      elim (Mem.fresh_block_alloc _ _ _ _ _ H0). eauto with mem.
+      apply memval_inject_incr with f; auto.
+  exists f'. split. constructor.
+(* inj *)
+  eapply Mem.alloc_left_mapped_inj; eauto. unfold f'; apply dec_eq_true.
+(* freeblocks *)
+  unfold f'; intros. destruct (eq_block b b1). subst b.
+  elim H9. eauto with mem.
+  eauto with mem.
+(* mappedblocks *)
+  unfold f'; intros. destruct (eq_block b b1). congruence. eauto.
+(* overlap *)
+  unfold f'; red; intros.
+  exploit Mem.perm_alloc_inv. eauto. eexact H12. intros P1.
+  exploit Mem.perm_alloc_inv. eauto. eexact H13. intros P2.
+  destruct (eq_block b0 b1); destruct (eq_block b3 b1).
+  congruence.
+  inversion H10; subst b0 b1' delta1.
+    destruct (eq_block b2 b2'); auto. subst b2'. right; red; intros.
+    eapply H6; eauto. lia.
+  inversion H11; subst b3 b2' delta2.
+    destruct (eq_block b1' b2); auto. subst b1'. right; red; intros.
+    eapply H6; eauto. lia.
+  eauto.
+(* representable *)
+  unfold f'; intros.
+  destruct (eq_block b b1).
+   subst. injection H9; intros; subst b' delta0. destruct H10.
+    exploit Mem.perm_alloc_inv; eauto; rewrite dec_eq_true; intro.
+    exploit H3. apply H4 with (k := Max) (p := Nonempty); eauto.
+    generalize (Ptrofs.unsigned_range_2 ofs). lia.
+   exploit Mem.perm_alloc_inv; eauto; rewrite dec_eq_true; intro.
+   exploit H3. apply H4 with (k := Max) (p := Nonempty); eauto.
+   generalize (Ptrofs.unsigned_range_2 ofs). lia.
+  eapply ma_representable0; try eassumption.
+  destruct H10; eauto using Mem.perm_alloc_4.
+(* incr *)
+  split. auto.
+(* image of b1 *)
+  split. unfold f'; apply dec_eq_true.
+(* image of others *)
+  intros. unfold f'; apply dec_eq_false; auto.
+Qed.
+
+Theorem alloc_right_inject:
+  forall f m1 m2 lo hi b2 m2',
+  magree f m1 m2 ->
+  Mem.alloc m2 lo hi = (m2', b2) ->
+  magree f m1 m2'.
+Proof.
+  intros. injection H0. intros NEXT MEM.
+  inversion H. constructor.
+(* inj *)
+  eapply Mem.alloc_right_inj; eauto.
+(* freeblocks *)
+  auto.
+(* mappedblocks *)
+  eauto with mem.
+(* no overlap *)
+  auto.
+(* representable *)
+  auto.
+Qed.
+
+Theorem alloc_parallel_inject:
+  forall f m1 m2 lo1 hi1 m1' b1 lo2 hi2,
+  magree f m1 m2 ->
+  Mem.alloc m1 lo1 hi1 = (m1', b1) ->
+  lo2 <= lo1 -> hi1 <= hi2 ->
+  exists f', exists m2', exists b2,
+  Mem.alloc m2 lo2 hi2 = (m2', b2)
+  /\ magree f' m1' m2'
+  /\ inject_incr f f'
+  /\ f' b1 = Some(b2, 0)
+  /\ (forall b, b <> b1 -> f' b = f b).
+Proof.
+  intros.
+  case_eq (Mem.alloc m2 lo2 hi2). intros m2' b2 ALLOC.
+  exploit alloc_left_mapped_inject.
+  eapply alloc_right_inject; eauto.
+  eauto.
+  instantiate (1 := b2). eauto with mem.
+  instantiate (1 := 0). unfold Ptrofs.max_unsigned. generalize Ptrofs.modulus_pos; lia.
+  auto.
+  intros. apply Mem.perm_implies with Freeable; auto with mem.
+  eapply Mem.perm_alloc_2; eauto. lia.
+  red; intros. apply Z.divide_0_r.
+  intros. apply (Mem.valid_not_valid_diff m2 b2 b2).
+  (* cannot solve by mem *)
+  eapply ma_mappedblocks;eauto.
+  eapply  Mem.fresh_block_alloc;eauto.
+  auto.
+ 
+  intros [f' [A [B [C D]]]].
+  exists f'; exists m2'; exists b2; auto.
+Qed.
+
+(** *End of A new injection *)
+
