assembler/RelocProgram.v
@@ -1,10 +1,3 @@
-(* *******************  *)
-(* Author: Yuting Wang  *)
-(*         Jinhua Wu    *)
-(* Date:   Sep 13, 2019 *)
-(* Last updated:  Feb 27, 2022 by Jinhua Wu*)
-(* *******************  *)
-
 (** * Template of languages with information about symbols and relocation *)
 
 Require Import Coqlib Maps Integers Values AST.
