x86/RelocProgGlobalenvs.v
@@ -1,0 +1,76 @@
+Require Import Coqlib Maps AST Integers Values.
+Require Import Events lib.Floats Memory Smallstep.
+Require Import Asm RelocProg RelocProgram Globalenvs.
+Require Import Locations Stacklayout Conventions.
+Require Import Linking Errors.
+Require Import LocalLib.
+
+(** Global environments using only the symbol table *)
+
+Definition gdef := globdef Asm.fundef unit.
+
+Module Genv.
+
+Section GENV.
+
+(* we use CompCert configuration technique to parameterize instruction type *)
+Record t: Type := mkgenv {
+  genv_symb: PTree.t (block * ptrofs);        (**r mapping symbol -> block * ptrofs *)
+  genv_ext_funs: NMap.t (option external_function);             (**r mapping blocks -> external function defintions *)
+  genv_instrs: NMap.t (ptrofs -> option instruction);    (**r mapping block  -> instructions mapping *)
+
+  genv_senv : Globalenvs.Senv.t; (**r symbol env *)
+}.
+
+(** ** Lookup functions *)
+
+Definition find_symbol (ge: t) (id: ident) : option (block * ptrofs):=
+  PTree.get id ge.(genv_symb).
+
+Definition symbol_address (ge: t) (id: ident) (ofs: ptrofs) : val :=
+  match find_symbol ge id with
+  | Some (b, o) => Vptr b (Ptrofs.add ofs o)
+  | None => Vundef
+  end.
+
+Definition find_ext_funct (ge: t) (v:val) : option external_function :=
+  match v with
+  | Vptr b ofs =>
+    if Ptrofs.eq ofs Ptrofs.zero then
+      NMap.get _ b ge.(genv_ext_funs)
+    else None
+  | _ => None
+  end.
+
+Lemma symbol_address_offset : forall ge ofs1 b s ofs,
+    symbol_address ge s Ptrofs.zero = Vptr b ofs ->
+    symbol_address ge s ofs1 = Vptr b (Ptrofs.add ofs ofs1).
+Proof.
+  unfold symbol_address. intros. 
+  destruct (find_symbol ge s) eqn:FSM.
+  - 
+    destruct p.
+    inv H.
+    rewrite Ptrofs.add_zero_l. rewrite Ptrofs.add_commut. auto.
+  - 
+    inv H.
+Qed.
+
+Lemma find_sym_to_addr : forall (ge:t) id b ofs,
+    find_symbol ge id = Some (b, ofs) ->
+    symbol_address ge id Ptrofs.zero = Vptr b ofs.
+Proof.
+  intros. unfold symbol_address. rewrite H.
+  rewrite Ptrofs.add_zero_l. auto.
+Qed.
+
+(** Find an instruction at an offset *)
+Definition find_instr (ge: t) (v:val) : option instruction :=
+  match v with
+  | Vptr b ofs => genv_instrs ge b ofs
+  | _ => None
+  end.
+
+End GENV.
+
+End Genv.
