x86/SymbtablegenArchi.v
@@ -1,0 +1,60 @@
+Require Import Coqlib Integers AST Maps.
+Require Import Asm.
+Require Import Errors.
+Require Import Memtype.
+Require Import RelocProg RelocProgram.
+Require Import CheckDef.
+Require Import LocalLib.
+Require Globalenvs.
+Import ListNotations.
+
+Set Implicit Arguments.
+
+Local Open Scope error_monad_scope.
+
+Definition instr_invalid (i: instruction) := 
+  match i with
+  | Pjmp_l _ 
+  | Pjcc _ _ 
+  | Pjcc2 _ _ _ 
+  (*Remove this instr after symbol table gen*)
+  | Pjmptbl _ _
+  | Pjmptbl_rel _ _
+  | Pallocframe _ _ _
+  | Pfreeframe _ _ _ => True
+  (* | Pload_parent_pointer _ _ _ => True *)
+  | _ => False
+  end.
+
+Definition instr_valid i := ~instr_invalid i.
+
+Lemma instr_invalid_dec: forall i, {instr_invalid i} + {~instr_invalid i}.
+Proof.
+  destruct i; cbn; auto.
+Qed.
+
+Lemma instr_valid_dec: forall i, {instr_valid i} + {~instr_valid i}.
+Proof.
+  unfold instr_valid.
+  destruct i; cbn; auto.
+Qed.
+
+Definition def_instrs_valid (def: (globdef fundef unit)) :=
+  match def with
+  | (Gvar v) => True
+  | (Gfun f) =>
+    match f with
+    | External _ => True
+    | Internal f =>  Forall instr_valid (fn_code f)
+    end
+  end.
+
+Lemma def_instrs_valid_dec: 
+  forall def, {def_instrs_valid def} + {~def_instrs_valid def}.
+Proof.
+  destruct def.
+  - destruct f. 
+    + simpl. apply Forall_dec. apply instr_valid_dec.
+    + simpl. auto.
+  - simpl. auto.
+Qed.
