x86/SymbtablegenproofArchi.v
@@ -1,0 +1,60 @@
+Require Import Coqlib Errors Maps.
+Require Import Integers Floats AST RelocProgLinking Linking.
+Require Import Values Memory Events Globalenvs Smallstep.
+Require Import Op Locations Mach Conventions Asm RealAsm.
+Require Import Symbtablegen SymbtablegenArchi.
+Require Import RelocProg RelocProgram RelocProgSemantics.
+Require Import LocalLib AsmInject.
+Import ListNotations.
+Require Import AsmFacts MemoryAgree.
+
+Section WITH_INSTR_SIZE.
+  Variable instr_size : instruction -> Z.
+  
+
+Lemma prog_instr_valid: forall prog tprog,
+    transf_program instr_size prog = OK tprog ->
+    Forall def_instrs_valid (map snd (AST.prog_defs prog)).
+Proof.
+  intros prog tprog TRANSF.
+  unfold transf_program in TRANSF.
+  destr_in TRANSF.
+  inv w. auto.
+Qed.
+
+(* TODEL *)
+Lemma int_funct_instr_valid: forall prog tprog f b,
+    transf_program instr_size prog = OK tprog ->
+    Globalenvs.Genv.find_funct_ptr (Genv.globalenv prog) b = Some (Internal f) ->
+    Forall instr_valid (Asm.fn_code f).
+Proof.
+  intros prog tprog f b TF FIND.
+  generalize (prog_instr_valid _ _ TF).
+  intros NJ.
+  generalize (Genv.find_funct_ptr_inversion _ _ FIND).
+  intros (id, IN).
+  generalize (in_map snd _ _ IN).
+  cbn. intros IN'.
+  rewrite Forall_forall in NJ.
+  apply NJ in IN'.
+  red in IN'. auto.
+Qed.
+
+(* TODEL *)
+Lemma instr_is_valid: forall prog tprog f b i ofs,
+    transf_program instr_size prog = OK tprog ->
+    Globalenvs.Genv.find_funct_ptr (Genv.globalenv prog) b = Some (Internal f) ->
+    Asm.find_instr instr_size ofs (Asm.fn_code f) = Some i ->
+    instr_valid i.
+Proof.
+  intros prog tprog f b i ofs TF FIND FIND'.
+  generalize (int_funct_instr_valid _ _ _ _ TF FIND).
+  intros NJ.
+  rewrite Forall_forall in NJ.
+  auto. 
+  apply NJ. 
+  eapply Asmgenproof0.find_instr_in; eauto.
+Qed.
+
+
+End WITH_INSTR_SIZE.
